\hdomi{START}{\plotbox{-1/3*(x+2)^2*x*(x-1)^2}{-5.5}{7.5}{-4.5}{7.5}}
\hdomi{$y=-\frac{1}{3}\cdot x\cdot (x+2)^2\cdot (x-1)^2$}{\plotbox{1/4*(x-2)^2*(x+3)^2}{-6.5}{6.5}{-1.5}{10.5}}
\hdomi{$y=\frac{1}{4}\cdot (x-2)^2\cdot (x+3)^2$}{\plotbox{-1/2*(x-2)^2*(x+1)}{-3.5}{3.5}{-3.5}{3.5}}
\hdomi{$y=-\frac{1}{2}\cdot (x-2)^2\cdot (x+1)$}{\plotbox{-1/4*(x-2)^2*(x+3)^2}{-6.5}{6.5}{-10.5}{1.5}}
\hdomi{$y=-\frac{1}{4}\cdot (x-2)^2\cdot (x+3)^2$}{\plotbox{1/3*x^2*(x+3)}{-7.5}{5.5}{-4.5}{7.5}}
\hdomi{$y=\frac{1}{3}\cdot x^2\cdot (x+3)$}{\plotbox{1/4*(x-1)*(x+3)^2}{-6.5}{6.5}{-5.5}{4.5}}
\hdomi{$y=\frac{1}{4}\cdot (x-1)\cdot (x+3)^2$}{\plotbox{-1/8*(x-1)^3*(x+3)^2}{-6.5}{6.5}{-4.5}{7.5}}
\hdomi{$y=-\frac{1}{3}\cdot (x-1)^3\cdot (x+3)^2$}{END}
